simplify
git-svn-id: https://projects.brucker.ch/hol-testgen/svn/HOL-TestGen/trunk/hol-testgen@11921 3260e6d1-4efc-4170-b0a7-36055960796d

src/compiler/meta/OCL_compiler_meta_Isabelle.thy
@@ -286,6 +286,8 @@ definition "Ty_arrow = Ty_apply_bin \<open>\<Rightarrow>\<close>"
 definition "Ty_times = Ty_apply_bin \<open>\<times>\<close>"
 definition "Consts' s l e = Consts_raw0 s (Ty_arrow (Ty_base \<open>'\<alpha>\<close>) l) e None"
 
+hide_const (open) insert
+hide_const (open) plus
 locale M
 begin
 definition "Method_simp_add_del l_a l_d = Method_simp_add_del_split l_a l_d []"
@@ -299,8 +301,8 @@ definition "intro = Method_intro"
 definition "elim = Method_elim"
 definition "subst_l0 = Method_subst"
 definition "subst_l = Method_subst_l"
-definition "insert' = Method_insert o List_map Thms_single"
-definition "plus' = Method_plus"
+definition "insert = Method_insert o List_map Thms_single"
+definition "plus = Method_plus"
 definition "option = Method_option"
 definition "or = Method_or"
 definition "meth_gen_simp = Method_simp_add_del [] []"
@@ -359,8 +361,8 @@ lemmas [code] =
   M.elim_def
   M.subst_l0_def
   M.subst_l_def
-  M.insert'_def
-  M.plus'_def
+  M.insert_def
+  M.plus_def
   M.option_def
   M.or_def
   M.meth_gen_simp_def
